Beginnings of DSE proof

coq/theories/Env.v
@@ -8,8 +8,10 @@ Section Env.
   Context `{K_eq_dec: EquivDec.EqDec K eq}.
   Definition t := list (K * V).
   Definition emp: t := [].
+  Definition diff_key (k: K) (b : K * V) :=
+    if K_eq_dec k (fst b) then false else true.
   Definition bind (k: K) (v: V) (e: t) : t :=
-    (k, v) :: e.
+    (k, v) :: filter (diff_key k) e.
   Fixpoint find (k: K) (e: t) : option V :=
     match e with
     | [] => None
@@ -18,4 +20,40 @@ Section Env.
       then Some v
       else find k s
     end.
+
+  Lemma diff_key_eq:
+    forall k v,
+      diff_key k (k, v) = false.
+  Proof.
+    intros.
+    cbv.
+    destruct (K_eq_dec k k); congruence.
+  Qed.
+
+  Lemma filter_idem:
+    forall A (f: A -> bool) l,
+      filter f (filter f l) = filter f l.
+  Proof.
+    induction l.
+    - reflexivity.
+    - simpl.
+      destruct (f a) eqn:?.
+      * simpl.
+        rewrite Heqb.
+        congruence.
+      * congruence.
+  Qed.
+
+  Lemma bind_overwrite:
+    forall e k v v',
+      bind k v' (bind k v e) = bind k v' e.
+  Proof.
+    unfold bind.
+    simpl.
+    intros.
+    rewrite diff_key_eq.
+    rewrite filter_idem.
+    reflexivity.
+  Qed.
+  
 End Env.
