coq/theories/LivenessProof.v
@@ -1,4 +1,5 @@
 Require Import Coq.Lists.List.
+Require Import Coq.micromega.Lia.
 Require Import MiniP4.Syntax.
 Require MiniP4.Env.
 Require Import MiniP4.Liveness.
@@ -6,9 +7,262 @@ Require Import MiniP4.Interp.
 Open Scope string_scope.
 Open Scope list_scope.
 
+Lemma check_union_false:
+  forall x a b,
+    check x (union a b) = false ->
+    check x a = false /\ check x b = false.
+Proof.
+Admitted.
+
 Definition dead (x: name) (c: cmd) : Prop :=
-  forall n s c s',
+  forall n s s',
     interp_cmd n s c = Some s' ->
     forall v,
       exists m,
-        interp_cmd m (assign s x v) = Some s'.
+        interp_cmd m (assign s x v) c = Some s'.
+
+Lemma exp_assign_fv:
+  forall s e x v,
+    check x (fv e) = false ->
+    interp_exp (assign s x v) e = interp_exp s e.
+Proof.
+  induction e.
+  simpl.
+Admitted.
+
+Lemma option_map_Some:
+  forall A B (f: A -> B) x y,
+    option_map f x = Some y ->
+    exists z,
+      x = Some z /\ y = f z.
+Proof.
+  unfold option_map.
+  intros.
+  destruct x.
+  - eexists.
+    intuition congruence.
+  - congruence.
+Qed.
+
+Lemma assign_overwrite:
+  forall s x v v',
+    assign (assign s x v) x v' = assign s x v'.
+Proof.
+  intros.
+  unfold assign, set_store; simpl.
+  rewrite Env.bind_overwrite.
+  tauto.
+Qed.
+
+Lemma check_cons_neq:
+  forall x y s,
+    x <> y ->
+    check x (y :: s) = check x s.
+Proof.
+  intros.
+  unfold check.
+  repeat destruct (in_dec _ _ _); try tauto.
+  - simpl in *.
+    intuition congruence.
+  - simpl in *.
+    tauto.
+Qed.
+
+Lemma check_cons_eq:
+  forall x s,
+    check x (x :: s) = true.
+Proof.
+  intros.
+  unfold check.
+  destruct (in_dec _ _ _); simpl in *; tauto.
+Qed.
+
+Lemma check_drop:
+  forall x y s,
+    x <> y ->
+    check x (drop y s) = check x s.
+Proof.
+  induction s; simpl; intros.
+  - reflexivity.
+  - unfold drop.
+    destruct (name_eq_dec y a), (name_eq_dec x a).
+    + congruence.
+    + rewrite check_cons_neq; auto.
+    + cbv in e; subst.
+      now rewrite !check_cons_eq.
+    + rewrite !check_cons_neq; auto.
+Qed.
+
+Lemma check_emp:
+  forall a,
+    check a emp = false.
+Proof.
+  unfold emp.
+  intros.
+  reflexivity.
+Qed.
+
+Lemma check_add_eq:
+  forall x s,
+    check x (add x s) = true.
+Proof.
+  intros.
+  unfold add.
+  destruct (check x s) eqn:?; [tauto|].
+  apply check_cons_eq.
+Qed.
+
+Lemma check_add_neq:
+  forall x y s,
+    x <> y ->
+    check x (add y s) = check x s.
+Proof.
+  intros.
+  unfold add.
+  destruct (check y s) eqn:?; [tauto|].
+  apply check_cons_neq.
+  tauto.
+Qed.
+
+Lemma union_emp_l:
+  forall s,
+    union emp s = s.
+Proof.
+  (* Not actually true, needs hypothesis about duplicates in s *)
+Admitted.
+
+Lemma interp_cmd_fuel:
+  forall m n s c v,
+    m >= n ->
+    interp_cmd n s c = Some v ->
+    interp_cmd m s c = Some v.
+Proof.
+Admitted.
+
+Lemma interp_extr_assign:
+  forall s x v t,
+    interp_extr (assign s x v) x t = interp_extr s x t.
+Proof.
+  intros.
+  unfold interp_extr.
+  simpl.
+  destruct (extr (pkt s) t) as [[? ?]|].
+  - rewrite Env.bind_overwrite.
+    reflexivity.
+  - reflexivity.
+Qed.
+
+Lemma dse_dead:
+  forall tables live c live' c',
+    dead_store_elim tables live c = (live', c') ->
+    forall x,
+      check x live' = false ->
+      dead x c \/ check x live = false.
+Proof.
+  induction c; simpl; intros.
+  - destruct (name_eq_dec x x0); unfold Equivalence.equiv in *; subst.
+    + destruct (check x0 live) eqn:?; inversion H; subst.
+      * apply check_union_false in H0; intuition.
+        left.
+        unfold dead; intros.
+        exists n.
+        destruct n; simpl in *; auto.
+        rewrite exp_assign_fv by auto.
+        eapply option_map_Some in H0.
+        destruct H0 as [z [? ?]].
+        subst.
+        rewrite H0.
+        simpl.
+        rewrite assign_overwrite.
+        reflexivity.
+      * tauto.
+    + right.
+      destruct (check x live) eqn:?; simpl in *.
+      * inversion H.
+        subst.
+        apply check_union_false in H0.
+        destruct H0 as [? ?].
+        rewrite check_drop in H0; eauto.
+      * congruence.
+  - admit.
+  - destruct (dead_store_elim tables live c1) as [live1 c1'] eqn:?.
+    destruct (dead_store_elim tables live c2) as [live2 c2'] eqn:?.
+    unfold union_all in *.
+    simpl in H.
+    inversion H; clear H.
+    subst live'.
+    subst c'.
+    specialize (IHc1 live1 c1' eq_refl x).
+    specialize (IHc2 live2 c2' eq_refl x).
+    apply check_union_false in H0.
+    destruct H0.
+    apply check_union_false in H.
+    destruct H.
+    apply IHc1 in H1.
+    apply IHc2 in H0.
+    intuition.
+    left.
+    rewrite union_emp_l in H.
+    unfold dead; intros.
+    destruct n; simpl in *; try congruence.
+    destruct (interp_exp s e) eqn:?; try congruence.
+    destruct (val_eq_dec v0 (VBits [true])) as [e0 | e0]; cbv in e0; subst.
+    * apply H2 in H0.
+      destruct (H0 v) as [m ?].
+      exists (S m).
+      destruct m; [cbn in *; congruence|].
+      remember (S m) as m'.
+      simpl.
+      rewrite exp_assign_fv; auto.
+      rewrite Heqo.
+      rewrite Heqm'.
+      eapply interp_cmd_fuel; [|eassumption].
+      lia.
+    * assert (interp_cmd n s c2 = Some s').
+      {
+        destruct v0; try congruence.
+        destruct bs as [|[|] [|?]]; try congruence.
+      }
+      clear H0.
+      apply H1 in H3.
+      destruct (H3 v) as [m ?].
+      exists (S m).
+      destruct m; [cbn in *; congruence|].
+      remember (S m) as m'.
+      simpl.
+      rewrite exp_assign_fv; auto.
+      rewrite Heqo.
+      cut (interp_cmd m' (assign s x v) c2 = Some s').
+      {
+        destruct v0; try congruence.
+        destruct bs as [|[|] [|?]]; try congruence.
+      }
+      rewrite Heqm'.
+      eapply interp_cmd_fuel; [|eassumption].
+      lia.
+  - inversion H.
+    subst.
+    clear H.
+    destruct (name_eq_dec x x0).
+    + cbv in e; subst x0.
+      left.
+      unfold dead; intros.
+      exists n.
+      destruct n; simpl in *; try congruence.
+      destruct (Env.find x (type_env s)) in *; try congruence.
+      rewrite interp_extr_assign.
+      tauto.
+    + right.
+      rewrite check_drop in H0; congruence.
+  - right.
+    destruct (name_eq_dec x x0).
+    + cbv in e; subst x0.
+      inversion H.
+      subst live'.
+      rewrite check_add_eq in *.
+      congruence.
+    + inversion H; subst live'.
+      rewrite check_add_neq in H0; eauto.
+  - admit.
+  - admit.
+Admitted.
